<?xml version="1.0" encoding="UTF-8"?>
<!DOCTYPE rdf:RDF [
  <!ENTITY cc "http://web.resource.org/cc/">
  <!ENTITY dcmi-terms "http://dublincore.org/documents/dcmi-terms/">
  <!ENTITY owl "http://www.w3.org/2002/07/owl#">
  <!ENTITY rdf "http://www.w3.org/1999/02/22-rdf-syntax-ns#">
  <!ENTITY rdfs "http://www.w3.org/2000/01/rdf-schema#">
  <!ENTITY reve "http://data.eurecom.fr/ontology/reve#">
  <!ENTITY terms "http://purl.org/dc/terms/">
  <!ENTITY vocab.sindice "http://vocab.sindice.net/">
  <!ENTITY xsd "http://www.w3.org/2001/XMLSchema#">
]>
<rdf:RDF xml:base="http://data.eurecom.fr/ontology/reve"
         xmlns:cc="http://web.resource.org/cc/"
         xmlns:dcmi-terms="http://dublincore.org/documents/dcmi-terms/"
         xmlns:owl="http://www.w3.org/2002/07/owl#"
         xmlns:rdf="http://www.w3.org/1999/02/22-rdf-syntax-ns#"
         xmlns:rdfs="http://www.w3.org/2000/01/rdf-schema#"
         xmlns:reve="http://data.eurecom.fr/ontology/reve#"
         xmlns:terms="http://purl.org/dc/terms/"
         xmlns:vocab.sindice="http://vocab.sindice.net/">

<!-- Ontology Information -->
  <owl:Ontology rdf:about=""
                terms:rights="Copyright 2012 EURECOM"
                owl:versionInfo="1.0">
    <dcmi-terms:created rdf:datatype="&xsd;date">2011-12-09</dcmi-terms:created>
    <dcmi-terms:title xml:lang="en">Research and Education Vocabulary for Eurecom</dcmi-terms:title>
    <terms:issued rdf:datatype="&xsd;date">2012-01-19</terms:issued>
    <rdf:type rdf:resource="&owl;Thing"/>
    <rdfs:comment xml:lang="en">An ontology to describe students, courses, publications and researchers at Eurecom</rdfs:comment>
    <rdfs:label xml:lang="en">Research and Education Vocabulary for EURECOM</rdfs:label>
  </owl:Ontology>

<!-- Classes -->
  <owl:Class rdf:about="#Alumnus">
    <rdfs:comment xml:lang="en">Holders of this role have graduated and received a PhD diploma or a Eurecom certificate</rdfs:comment>
    <rdfs:comment xml:lang="fr">Les titulaires de ce rôle ont fini un cursus à Eurecom et détiennent un diplôme de doctorat ou une certification Eurecom</rdfs:comment>
    <rdfs:isDefinedBy rdf:resource="http://data.eurecom.fr/ontology/"/>
    <rdfs:label xml:lang="en">Alumnus</rdfs:label>
    <rdfs:label xml:lang="fr">Ancien élève</rdfs:label>
    <rdfs:subClassOf rdf:resource="http://purl.org/vocab/aiiso-roles/schema#Role"/>
  </owl:Class>

  <owl:Class rdf:about="#Attendee">
    <rdfs:comment xml:lang="en">Holders of this role have registered for one or several courses</rdfs:comment>
    <rdfs:comment xml:lang="fr">Les titulaires de ce rôle sont inscrits à un ou plusieurs cours</rdfs:comment>
    <rdfs:isDefinedBy rdf:resource="http://data.eurecom.fr/ontology/"/>
    <rdfs:label xml:lang="en">Attendee</rdfs:label>
    <rdfs:label xml:lang="fr">Participant</rdfs:label>
    <rdfs:subClassOf rdf:resource="http://purl.org/vocab/aiiso-roles/schema#Role"/>
  </owl:Class>

  <owl:Class rdf:about="#Course">
    <rdfs:comment xml:lang="en">A teaching unit. A course is composed of several course sessions.</rdfs:comment>
    <rdfs:comment xml:lang="fr">Une unité d'enseignement. Un cours est composé de plusieurs sessions de cours.</rdfs:comment>
    <rdfs:isDefinedBy rdf:resource="http://data.eurecom.fr/ontology/"/>
    <rdfs:label xml:lang="fr">Cours</rdfs:label>
    <rdfs:label xml:lang="en">Course</rdfs:label>
    <owl:equivalentClass rdf:resource="http://purl.org/vocab/aiiso/schema#Course"/>
  </owl:Class>

  <owl:Class rdf:about="#CourseCreditForTrack">
    <rdfs:comment xml:lang="en">A container for n-ary relationship for Course, Track and credits number.</rdfs:comment>
    <rdfs:comment xml:lang="fr">Un contenant de la relation n-aire pour le cours, la filière et le nombre de crédits.</rdfs:comment>
    <rdfs:label xml:lang="en">Course credit for track.</rdfs:label>
    <rdfs:label xml:lang="fr">Crédit du cours pour la filière.</rdfs:label>
  </owl:Class>

  <owl:Class rdf:about="#CourseSession">
    <rdfs:comment xml:lang="en">A course session is a ponctual event on which teacher and students gather, for a given course.</rdfs:comment>
    <rdfs:comment xml:lang="fr">Une session de cours est un évènement ponctuel qui rassemble professeur et élèves en un lieu donné, au sujet d'un cours.</rdfs:comment>
    <rdfs:isDefinedBy rdf:resource="http://data.eurecom.fr/ontology/"/>
    <rdfs:label xml:lang="en">Course session</rdfs:label>
    <rdfs:label xml:lang="fr">Session de cours</rdfs:label>
    <rdfs:subClassOf rdf:resource="http://linkedevents.org/ontology/Event"/>
  </owl:Class>

  <owl:Class rdf:about="#Curriculum">
    <rdfs:comment xml:lang="en">A curriculum is a title of a training period offered at Eurecom which consists of credits compatible with the LMD European standard.
Eurecom supports four types of curriculum, which is Engineering, Master of science, Post Master degree and doctoral program.</rdfs:comment>
    <rdfs:comment xml:lang="fr">Une formation est une période d'étude proposée par Eurecom comprenant des crédits compatibles au système LMD
Eurecom propose quatre types of formation, qui sont ingénieurie, master international, ingénieur de spécialisation et le programme doctoral. </rdfs:comment>
    <rdfs:label xml:lang="en">Curriculum</rdfs:label>
    <rdfs:label xml:lang="fr">Formation</rdfs:label>
  </owl:Class>

  <owl:Class rdf:about="#DoctoralStudent">
    <rdfs:comment xml:lang="en">Holders of this role are students doing a PhD thesis.</rdfs:comment>
    <rdfs:comment xml:lang="fr">Les titulaires de ce rôle sont les étudiants effectuant une thèse de doctorat.</rdfs:comment>
    <rdfs:isDefinedBy rdf:resource="http://data.eurecom.fr/ontology/"/>
    <rdfs:label xml:lang="en">Doctoral student</rdfs:label>
    <rdfs:label xml:lang="fr">Doctorant</rdfs:label>
    <rdfs:subClassOf rdf:resource="http://purl.org/vocab/aiiso-roles/schema#Role"/>
  </owl:Class>

  <owl:Class rdf:about="#GeneralCourse">
    <rdfs:comment xml:lang="en">A course which brings knowledge in law, economy, or management</rdfs:comment>
    <rdfs:comment xml:lang="fr">Un cours qui apporte des connaissances en droit, en économie, ou en gestion</rdfs:comment>
    <rdfs:isDefinedBy rdf:resource="http://data.eurecom.fr/ontology/"/>
    <rdfs:label xml:lang="fr">Cours d'enseignement général</rdfs:label>
    <rdfs:label xml:lang="en">General course</rdfs:label>
    <rdfs:subClassOf rdf:resource="#Course"/>
    <owl:disjointWith rdf:resource="#LanguageCourse"/>
    <owl:disjointWith rdf:resource="#TechnicalCourse"/>
  </owl:Class>

  <owl:Class rdf:about="#LanguageCourse">
    <rdfs:comment xml:lang="en">A course in which one learns a language other than one's native language</rdfs:comment>
    <rdfs:comment xml:lang="fr">Un cours où l'on apprend à s'exprimer dans une autre langue que la sienne</rdfs:comment>
    <rdfs:isDefinedBy rdf:resource="http://data.eurecom.fr/ontology/"/>
    <rdfs:label xml:lang="fr">Cours de langue</rdfs:label>
    <rdfs:label xml:lang="en">Language course</rdfs:label>
    <rdfs:subClassOf rdf:resource="#Course"/>
    <owl:disjointWith rdf:resource="#GeneralCourse"/>
    <owl:disjointWith rdf:resource="#TechnicalCourse"/>
  </owl:Class>

  <owl:Class rdf:about="#ResearchUnit">
    <rdfs:comment xml:lang="en">A Research Unit is a group dedicated to research at Eurecom, and there are three of them.</rdfs:comment>
    <rdfs:comment xml:lang="fr">Une unité de recherche est un groupe dédié à la recherche à Eurecom. Il y en a trois.</rdfs:comment>
    <rdfs:isDefinedBy rdf:resource="http://data.eurecom.fr/ontology/"/>
    <rdfs:label xml:lang="en">Research unit</rdfs:label>
    <rdfs:label xml:lang="fr">Unité de recherche</rdfs:label>
    <rdfs:subClassOf rdf:resource="http://xmlns.com/foaf/0.1/Group"/>
    <owl:equivalentClass rdf:resource="http://purl.org/vocab/aiiso/schema#ResearchGroup"/>
  </owl:Class>

  <owl:Class rdf:about="#Researcher">
    <rdfs:comment xml:lang="en">Holders of this role do research.</rdfs:comment>
    <rdfs:comment xml:lang="fr">Les titulaires de ce rôle effectuent des recherches.</rdfs:comment>
    <rdfs:isDefinedBy rdf:resource="http://data.eurecom.fr/ontology/"/>
    <rdfs:label xml:lang="fr">Chercheur</rdfs:label>
    <rdfs:label xml:lang="en">Researcher</rdfs:label>
    <rdfs:subClassOf rdf:resource="http://purl.org/vocab/aiiso-roles/schema#Role"/>
    <owl:disjointWith rdf:resource="#Student"/>
  </owl:Class>

  <owl:Class rdf:about="#Semester">
    <rdfs:comment xml:lang="en">A semester, from the administrative point of view : it typically ranges from the beginning of October to the middle of February, or from the beginning of March to the end of June. It has a catalog of courses attached to it.</rdfs:comment>
    <rdfs:comment xml:lang="fr">Un semestre, du point de vue administratif : typiquement, il s'étend du début du mois d'octobre à la mi-février, ou bien de mars à la fin juin. Un catalogue de cours y est rattaché.</rdfs:comment>
    <rdfs:isDefinedBy rdf:resource="http://data.eurecom.fr/ontology/"/>
    <rdfs:label xml:lang="en">Semester</rdfs:label>
    <rdfs:label xml:lang="fr">Semestre</rdfs:label>
  </owl:Class>

  <owl:Class rdf:about="#Staff">
    <rdfs:comment xml:lang="en">Holders of this role receive a salary from Eurecom.</rdfs:comment>
    <rdfs:comment xml:lang="fr">Les titulaires de ce rôle reçoivent un salaire d'Eurecom.</rdfs:comment>
    <rdfs:isDefinedBy rdf:resource="http://data.eurecom.fr/ontology/"/>
    <rdfs:label xml:lang="fr">Employé</rdfs:label>
    <rdfs:label xml:lang="en">Staff</rdfs:label>
    <rdfs:subClassOf rdf:resource="http://purl.org/vocab/aiiso-roles/schema#Role"/>
  </owl:Class>

  <owl:Class rdf:about="#Student">
    <rdfs:comment xml:lang="en">Holders of this role are enrolled at a university.</rdfs:comment>
    <rdfs:comment xml:lang="fr">Les titulaires de ce rôle sont engagés dans un cursus d'enseignement supérieur.</rdfs:comment>
    <rdfs:isDefinedBy rdf:resource="http://data.eurecom.fr/ontology/"/>
    <rdfs:label xml:lang="fr">Etudiant</rdfs:label>
    <rdfs:label xml:lang="en">Student</rdfs:label>
    <rdfs:subClassOf rdf:resource="http://purl.org/vocab/aiiso-roles/schema#Role"/>
    <owl:disjointWith rdf:resource="#Researcher"/>
    <owl:disjointWith rdf:resource="#Teacher"/>
  </owl:Class>

  <owl:Class rdf:about="#Teacher">
    <rdfs:comment xml:lang="en">Holders of this role teach one or several courses.</rdfs:comment>
    <rdfs:comment xml:lang="fr">Les titulaires de ce rôle enseignent un ou plusieurs cours.</rdfs:comment>
    <rdfs:isDefinedBy rdf:resource="http://data.eurecom.fr/ontology/"/>
    <rdfs:label xml:lang="fr">Enseignant</rdfs:label>
    <rdfs:label xml:lang="en">Teacher</rdfs:label>
    <rdfs:subClassOf rdf:resource="http://purl.org/vocab/aiiso-roles/schema#Role"/>
    <owl:disjointWith rdf:resource="#Student"/>
  </owl:Class>

  <owl:Class rdf:about="#TechnicalCourse">
    <rdfs:comment xml:lang="en">A course which brings scientific knowledge in one of the domains of expertise of Eurecom</rdfs:comment>
    <rdfs:comment xml:lang="fr">Un cours qui apporte des connaissances scientifiques dans l'un des domaines d'expertise d'Eurecom.</rdfs:comment>
    <rdfs:isDefinedBy rdf:resource="http://data.eurecom.fr/ontology/"/>
    <rdfs:label xml:lang="fr">Cours d'enseignement technique</rdfs:label>
    <rdfs:label xml:lang="en">Technical course</rdfs:label>
    <rdfs:subClassOf rdf:resource="#Course"/>
    <owl:disjointWith rdf:resource="#GeneralCourse"/>
    <owl:disjointWith rdf:resource="#LanguageCourse"/>
  </owl:Class>

  <owl:Class rdf:about="#Track">
    <rdfs:comment xml:lang="en">A set of mandatory and optional courses, built around a common domain. To help students select their courses, the curriculum is organized around 7 teaching tracks. Each track includes core courses, restrictive elective courses, and free elective courses that students are entirely free to choose from (except for languages).</rdfs:comment>
    <rdfs:comment xml:lang="fr">Un ensemble de cours obligatoires et optionnels, contruit autour d'un même domaine. Pour aider les étudiants à choisir leur cours, le cursus est organisé autour de 7 filières d'enseignement. Chaque filière comprend des cours obligatoires, des cours à choisir dans un menu et des cours à choix entièrement libres (à l'exception des cours de langues vivantes).</rdfs:comment>
    <rdfs:isDefinedBy rdf:resource="http://data.eurecom.fr/ontology/"/>
    <rdfs:label xml:lang="fr">Filière</rdfs:label>
    <rdfs:label xml:lang="en">Track</rdfs:label>
    <rdfs:subClassOf rdf:resource="http://purl.org/vocab/aiiso/schema#KnowledgeGrouping"/>
  </owl:Class>

  <owl:Class rdf:about="#VisitingScientist">
    <rdfs:comment xml:lang="en">Holders of this role are researchers welcomed at Eurecom for a certain duration</rdfs:comment>
    <rdfs:comment xml:lang="fr">Les titulaires de ce rôle sont des chercheurs reçus à Eurecom pour une durée déterminée</rdfs:comment>
    <rdfs:isDefinedBy rdf:resource="http://data.eurecom.fr/ontology/"/>
    <rdfs:label xml:lang="fr">Visiteur scientifique</rdfs:label>
    <rdfs:label xml:lang="en">Visiting scientist</rdfs:label>
    <rdfs:subClassOf rdf:resource="http://purl.org/vocab/aiiso-roles/schema#Role"/>
  </owl:Class>

  <owl:Class rdf:about="http://linkedevents.org/ontology/Event"/>
  <owl:Class rdf:about="http://purl.org/vocab/aiiso-roles/schema#Role"/>
  <owl:Class rdf:about="http://purl.org/vocab/aiiso/schema#Course"/>
  <owl:Class rdf:about="http://purl.org/vocab/aiiso/schema#KnowledgeGrouping"/>
  <owl:Class rdf:about="http://purl.org/vocab/aiiso/schema#ResearchGroup"/>
  <owl:Class rdf:about="&cc;License"/>
  <owl:Class rdf:about="&cc;Work"/>
  <owl:Class rdf:about="http://xmlns.com/foaf/0.1/Document"/>
  <owl:Class rdf:about="http://xmlns.com/foaf/0.1/Group"/>
  <owl:Class rdf:about="http://xmlns.com/foaf/0.1/Person"/>

<!-- Datatypes -->
  <rdfs:Datatype rdf:about="&xsd;float"/>

<!-- Annotation Properties -->
  <owl:AnnotationProperty rdf:about="&rdfs;comment"/>
  <owl:AnnotationProperty rdf:about="&rdfs;isDefinedBy"/>
  <owl:AnnotationProperty rdf:about="&rdfs;label"/>
  <owl:AnnotationProperty rdf:about="&owl;versionInfo"/>

<!-- Datatype Properties -->
  <owl:DatatypeProperty rdf:about="#hasCredit">
    <rdfs:comment xml:lang="fr">Attribut faisant référence au nombre de crédits dans la relation (cours, crédit, filière).</rdfs:comment>
    <rdfs:comment xml:lang="en">Data type property referencing the number of credits in the (course, credit, track) relationship.</rdfs:comment>
    <rdfs:domain rdf:resource="#CourseCreditForTrack"/>
    <rdfs:label xml:lang="fr">crédit</rdfs:label>
    <rdfs:label xml:lang="en">has credit</rdfs:label>
    <rdfs:range rdf:resource="&xsd;float"/>
  </owl:DatatypeProperty>

  <owl:DatatypeProperty rdf:about="#referenceAtEurecom">
    <rdfs:comment xml:lang="en">An article's reference in Eurecom's bibliographic repository.</rdfs:comment>
    <rdfs:comment xml:lang="fr">La référence d'un article dans la base bibliographique d'Eurecom.</rdfs:comment>
    <rdfs:domain rdf:resource="http://xmlns.com/foaf/0.1/Document"/>
    <rdfs:isDefinedBy rdf:resource="http://data.eurecom.fr/ontology/"/>
    <rdfs:label xml:lang="en">reference at Eurecom</rdfs:label>
    <rdfs:label xml:lang="fr">référence Eurecom</rdfs:label>
  </owl:DatatypeProperty>

  <owl:DatatypeProperty rdf:about="&dcmi-terms;created"/>
  <owl:DatatypeProperty rdf:about="&dcmi-terms;title"/>
  <owl:DatatypeProperty rdf:about="&terms;issued"/>
  <owl:DatatypeProperty rdf:about="&terms;rights"/>
  <owl:DatatypeProperty rdf:about="&vocab.sindice;date"/>
  <owl:DatatypeProperty rdf:about="&vocab.sindice;size"/>

<!-- Object Properties -->
  <owl:ObjectProperty rdf:about="#availableDuring">
    <rdfs:comment xml:lang="en">Property referencing a semester during which the course is available</rdfs:comment>
    <rdfs:comment xml:lang="fr">Propriété faisant référence à un semestre pendant lequel le cours est disponible</rdfs:comment>
    <rdfs:domain rdf:resource="#Course"/>
    <rdfs:isDefinedBy rdf:resource="http://data.eurecom.fr/ontology/"/>
    <rdfs:label xml:lang="en">available during</rdfs:label>
    <rdfs:label xml:lang="fr">disponible pendant</rdfs:label>
    <rdfs:range rdf:resource="#Semester"/>
    <owl:inverseOf rdf:resource="#hasAvailableCourse"/>
  </owl:ObjectProperty>

  <owl:ObjectProperty rdf:about="#hasAvailableCourse">
    <rdfs:comment xml:lang="en">Property referencing a course available during the semester</rdfs:comment>
    <rdfs:comment xml:lang="fr">Propriété faisant référence à un cours disponible pendant le semestre</rdfs:comment>
    <rdfs:domain rdf:resource="#Semester"/>
    <rdfs:isDefinedBy rdf:resource="http://data.eurecom.fr/ontology/"/>
    <rdfs:label xml:lang="fr">a comme cours disponible</rdfs:label>
    <rdfs:label xml:lang="en">has available course</rdfs:label>
    <rdfs:range rdf:resource="#Course"/>
    <owl:inverseOf rdf:resource="#availableDuring"/>
  </owl:ObjectProperty>

  <owl:ObjectProperty rdf:about="#hasConstituent">
    <rdfs:comment xml:lang="en">A course consists in several course sessions</rdfs:comment>
    <rdfs:comment xml:lang="fr">Un cours est constitué de plusieurs sessions de cours</rdfs:comment>
    <rdfs:domain rdf:resource="#Course"/>
    <rdfs:isDefinedBy rdf:resource="http://data.eurecom.fr/ontology/"/>
    <rdfs:label xml:lang="fr">a pour constituant</rdfs:label>
    <rdfs:label xml:lang="en">has constituent</rdfs:label>
    <rdfs:range rdf:resource="#CourseSession"/>
    <owl:inverseOf rdf:resource="#isConstituentOf"/>
  </owl:ObjectProperty>

  <owl:ObjectProperty rdf:about="#hasCoordinator">
    <rdfs:comment xml:lang="en">Property referencing a person responsible for the track</rdfs:comment>
    <rdfs:comment xml:lang="fr">Propriété faisant référence à une personne responsable de la filière</rdfs:comment>
    <rdfs:domain rdf:resource="#Track"/>
    <rdfs:isDefinedBy rdf:resource="http://data.eurecom.fr/ontology/"/>
    <rdfs:label xml:lang="fr">a pour coordinateur</rdfs:label>
    <rdfs:label xml:lang="en">has coordinator</rdfs:label>
    <rdfs:range rdf:resource="http://xmlns.com/foaf/0.1/Person"/>
    <owl:inverseOf rdf:resource="#isCoordinatorOf"/>
  </owl:ObjectProperty>

  <owl:ObjectProperty rdf:about="#hasCreditForTrack">
    <rdfs:comment xml:lang="en">Property referencing to the credits for the successful completion of the course in a given track.</rdfs:comment>
    <rdfs:comment xml:lang="fr">Propriété faisant référence au nombre de crédits reçus pour la validation du cours dans une filière donnée.</rdfs:comment>
    <rdfs:domain rdf:resource="#Course"/>
    <rdfs:label xml:lang="fr">Crédit pour la filière</rdfs:label>
    <rdfs:label xml:lang="en">has credit for track</rdfs:label>
    <rdfs:range rdf:resource="#CourseCreditForTrack"/>
    <owl:inverseOf rdf:resource="#isCreditForCourse"/>
  </owl:ObjectProperty>

  <owl:ObjectProperty rdf:about="#hasDuration">
    <rdfs:comment xml:lang="en">Property referencing a semester in the curriculum.</rdfs:comment>
    <rdfs:domain rdf:resource="#Curriculum"/>
    <rdfs:label xml:lang="en">has duration</rdfs:label>
    <rdfs:range rdf:resource="#Semester"/>
    <owl:inverseOf rdf:resource="#isDurationOf"/>
  </owl:ObjectProperty>

  <owl:ObjectProperty rdf:about="#hasFreeCourse">
    <rdfs:comment xml:lang="en">Property referencing a course considered free for the track</rdfs:comment>
    <rdfs:domain rdf:resource="#Track"/>
    <rdfs:label xml:lang="en">has free course</rdfs:label>
    <rdfs:range rdf:resource="#Course"/>
    <owl:inverseOf rdf:resource="#isFreeFor"/>
  </owl:ObjectProperty>

  <owl:ObjectProperty rdf:about="#hasMandatoryCourse">
    <rdfs:comment xml:lang="en">Property referencing a course considered mandatory for the track</rdfs:comment>
    <rdfs:comment xml:lang="fr">Propriété faisant référence à un cours considéré comme obligatoire pour la filière</rdfs:comment>
    <rdfs:domain rdf:resource="#Track"/>
    <rdfs:isDefinedBy rdf:resource="http://data.eurecom.fr/ontology/"/>
    <rdfs:label xml:lang="fr">a comme cours obligatoire</rdfs:label>
    <rdfs:label xml:lang="en">has mandatory course</rdfs:label>
    <rdfs:range rdf:resource="#Course"/>
    <owl:inverseOf rdf:resource="#isMandatoryFor"/>
  </owl:ObjectProperty>

  <owl:ObjectProperty rdf:about="#hasOptionalCourse">
    <rdfs:comment xml:lang="en">Property referencing a course considered optional for the track</rdfs:comment>
    <rdfs:comment xml:lang="fr">Propriété faisant référence à un cours considéré comme optionnel pour la filière</rdfs:comment>
    <rdfs:domain rdf:resource="#Track"/>
    <rdfs:isDefinedBy rdf:resource="http://data.eurecom.fr/ontology/"/>
    <rdfs:label xml:lang="fr">a comme cours optionnel</rdfs:label>
    <rdfs:label xml:lang="en">has optional course</rdfs:label>
    <rdfs:range rdf:resource="#Course"/>
    <owl:inverseOf rdf:resource="#isOptionalFor"/>
  </owl:ObjectProperty>

  <owl:ObjectProperty rdf:about="#hasTrack">
    <rdfs:comment xml:lang="en">Property referencing to a track in the (course, credit, track) relationship.</rdfs:comment>
    <rdfs:comment xml:lang="fr">Propriété faisant référence à la filière dans la relation (cours, crédit, filière).</rdfs:comment>
    <rdfs:domain rdf:resource="#CourseCreditForTrack"/>
    <rdfs:label xml:lang="fr">filière</rdfs:label>
    <rdfs:label xml:lang="en">has track</rdfs:label>
    <rdfs:range rdf:resource="#Track"/>
    <owl:inverseOf rdf:resource="#isTrackOf"/>
  </owl:ObjectProperty>

  <owl:ObjectProperty rdf:about="#isConstituentOf">
    <rdfs:comment xml:lang="en">A course consists in several course sessions</rdfs:comment>
    <rdfs:comment xml:lang="fr">Un cours est constitué de plusieurs sessions de cours</rdfs:comment>
    <rdfs:domain rdf:resource="#CourseSession"/>
    <rdfs:isDefinedBy rdf:resource="http://data.eurecom.fr/ontology/"/>
    <rdfs:label xml:lang="fr">est un constituant de</rdfs:label>
    <rdfs:label xml:lang="en">is constituent of</rdfs:label>
    <rdfs:range rdf:resource="#Course"/>
    <owl:inverseOf rdf:resource="#hasConstituent"/>
  </owl:ObjectProperty>

  <owl:ObjectProperty rdf:about="#isCoordinatorOf">
    <rdfs:comment xml:lang="en">Property referencing a track the person is responsible for</rdfs:comment>
    <rdfs:comment xml:lang="fr">Propriété faisant référence à une filière dont la personne est responsable</rdfs:comment>
    <rdfs:domain rdf:resource="http://xmlns.com/foaf/0.1/Person"/>
    <rdfs:isDefinedBy rdf:resource="http://data.eurecom.fr/ontology/"/>
    <rdfs:label xml:lang="fr">est le coordinateur de</rdfs:label>
    <rdfs:label xml:lang="en">is coordinator of</rdfs:label>
    <rdfs:range rdf:resource="#Track"/>
    <owl:inverseOf rdf:resource="#hasCoordinator"/>
  </owl:ObjectProperty>

  <owl:ObjectProperty rdf:about="#isCreditForCourse">
    <rdfs:comment xml:lang="en">Property referencing the course in the (course, credit, track) relationship.</rdfs:comment>
    <rdfs:comment xml:lang="fr">Propriété faisant référence au cours dans la relation (cours, crédit, filière).</rdfs:comment>
    <rdfs:domain rdf:resource="#CourseCreditForTrack"/>
    <rdfs:label xml:lang="fr">est le crédit pour le cours</rdfs:label>
    <rdfs:label xml:lang="en">is credit for course</rdfs:label>
    <rdfs:range rdf:resource="#Course"/>
    <owl:inverseOf rdf:resource="#hasCreditForTrack"/>
  </owl:ObjectProperty>

  <owl:ObjectProperty rdf:about="#isDurationOf">
    <rdfs:comment xml:lang="en">Property referencing to a curriculum for which the semester is included</rdfs:comment>
    <rdfs:domain rdf:resource="#Semester"/>
    <rdfs:label xml:lang="en">is duration of</rdfs:label>
    <rdfs:range rdf:resource="#Curriculum"/>
  </owl:ObjectProperty>

  <owl:ObjectProperty rdf:about="#isFreeFor">
    <rdfs:comment xml:lang="en">Property referencing a track for which the course is considered free.</rdfs:comment>
    <rdfs:domain rdf:resource="#Course"/>
    <rdfs:label xml:lang="en">is free for</rdfs:label>
    <rdfs:range rdf:resource="#Track"/>
  </owl:ObjectProperty>

  <owl:ObjectProperty rdf:about="#isMandatoryFor">
    <rdfs:comment xml:lang="en">Property referencing a track for which the course is considered mandatory</rdfs:comment>
    <rdfs:comment xml:lang="fr">Propriété faisant référence à une filière pour laquelle le cours est considéré comme obligatoire</rdfs:comment>
    <rdfs:domain rdf:resource="#Course"/>
    <rdfs:isDefinedBy rdf:resource="http://data.eurecom.fr/ontology/"/>
    <rdfs:label xml:lang="fr">est obligatoire pour</rdfs:label>
    <rdfs:label xml:lang="en">is mandatory for</rdfs:label>
    <rdfs:range rdf:resource="#Track"/>
    <owl:inverseOf rdf:resource="#hasMandatoryCourse"/>
  </owl:ObjectProperty>

  <owl:ObjectProperty rdf:about="#isOptionalFor">
    <rdfs:comment xml:lang="en">Property referencing a track for which the course is considered optional</rdfs:comment>
    <rdfs:comment xml:lang="fr">Propriété faisant référence à une filière pour laquelle le cours est considéré comme optionnel</rdfs:comment>
    <rdfs:domain rdf:resource="#Course"/>
    <rdfs:isDefinedBy rdf:resource="http://data.eurecom.fr/ontology/"/>
    <rdfs:label xml:lang="fr">est optionnel pour</rdfs:label>
    <rdfs:label xml:lang="en">is optional for</rdfs:label>
    <rdfs:range rdf:resource="#Track"/>
    <owl:inverseOf rdf:resource="#hasOptionalCourse"/>
  </owl:ObjectProperty>

  <owl:ObjectProperty rdf:about="#isTrackOf">
    <rdfs:comment xml:lang="en">Property referencing to a (course, credit, track) relationship the track is involved in.</rdfs:comment>
    <rdfs:comment xml:lang="fr">Propriété faisant référence à une relation (cours, crédit, filière) dans laquelle la filière est impliquée.</rdfs:comment>
    <rdfs:domain rdf:resource="#Track"/>
    <rdfs:label xml:lang="fr">est la filière de</rdfs:label>
    <rdfs:label xml:lang="en">is track of</rdfs:label>
    <rdfs:range rdf:resource="#CourseCreditForTrack"/>
  </owl:ObjectProperty>

  <owl:ObjectProperty rdf:about="&terms;type"/>
  <owl:ObjectProperty rdf:about="&cc;license"/>
  <owl:ObjectProperty rdf:about="&cc;permits"/>
  <owl:ObjectProperty rdf:about="&cc;requires"/>

<!-- Instances -->
  <reve:Curriculum rdf:about="#doctoralProgram"
                   rdfs:label="doctoral program"/>
  <reve:GeneralCourse rdf:about="#economy">
    <rdfs:comment xml:lang="en">One matter of the non-technical courses</rdfs:comment>
    <rdfs:label xml:lang="en">economy</rdfs:label>
  </reve:GeneralCourse>

  <reve:Curriculum rdf:about="#engineering"
                   rdfs:label="engineering"/>
  <reve:Semester rdf:about="#fall1"
                 rdfs:label="fall1">
    <rdfs:comment>The first semester of engineering program.</rdfs:comment>
  </reve:Semester>

  <reve:Semester rdf:about="#fall2"
                 rdfs:label="fall2">
    <rdfs:comment>The third semester of engineering program.</rdfs:comment>
  </reve:Semester>

  <reve:GeneralCourse rdf:about="#humanSciences">
    <rdfs:comment xml:lang="en">One matter of the non-technical course</rdfs:comment>
    <rdfs:label xml:lang="en">Human Sciences</rdfs:label>
  </reve:GeneralCourse>

  <reve:Semester rdf:about="#internship"
                 rdfs:label="inter">
    <rdfs:comment>The internship semester of engineering program.</rdfs:comment>
  </reve:Semester>

  <reve:GeneralCourse rdf:about="#law">
    <rdfs:comment xml:lang="en">One matter of the non-technical course</rdfs:comment>
    <rdfs:label xml:lang="en">law</rdfs:label>
  </reve:GeneralCourse>

  <reve:Curriculum rdf:about="#masterOfScience"
                   rdfs:label="master of science"/>
  <reve:Curriculum rdf:about="#postMaster"
                   rdfs:label="post master"/>
  <reve:GeneralCourse rdf:about="#projectManagement">
    <rdfs:comment xml:lang="en">One matter of the non-technical course</rdfs:comment>
    <rdfs:label xml:lang="en">Project Management</rdfs:label>
  </reve:GeneralCourse>

  <reve:Semester rdf:about="#spring"
                 rdfs:label="spring">
    <rdfs:comment>The second semester of engineering program.</rdfs:comment>
  </reve:Semester>

  <cc:Work rdf:about="file:/C:/Users/Ghislain/Documents/Ghislain/data-eurecom-fr/REVE%20ontology/reve_1.0.rdf">
    <terms:type rdf:resource="http://purl.org/dc/dcmitype/Text"/>
    <cc:license rdf:resource="http://creativecommons.org/licenses/by/1.0/"/>
  </cc:Work>

  <owl:Thing rdf:about="http://any23.org/tmp/"
             vocab.sindice:date="2012-01-19T15:48:03+00:00">
    <vocab.sindice:size rdf:datatype="&xsd;int">296</vocab.sindice:size>
  </owl:Thing>

  <cc:License rdf:about="http://creativecommons.org/licenses/by/1.0/">
    <cc:permits rdf:resource="&cc;DerivativeWorks"/>
    <cc:permits rdf:resource="&cc;Distribution"/>
    <cc:permits rdf:resource="&cc;Reproduction"/>
    <cc:requires rdf:resource="&cc;Attribution"/>
    <cc:requires rdf:resource="&cc;Notice"/>
  </cc:License>

  <owl:Thing rdf:about="http://purl.org/dc/dcmitype/Text"/>
  <owl:Thing rdf:about="&cc;Attribution"/>
  <owl:Thing rdf:about="&cc;DerivativeWorks"/>
  <owl:Thing rdf:about="&cc;Distribution"/>
  <owl:Thing rdf:about="&cc;Notice"/>
  <owl:Thing rdf:about="&cc;Reproduction"/>
</rdf:RDF>
