<?xml version="1.0"?>


<!DOCTYPE rdf:RDF [
    <!ENTITY terms "http://purl.org/dc/terms/" >
    <!ENTITY vocab.sindice "http://vocab.sindice.net/" >
    <!ENTITY cc "http://web.resource.org/cc/" >
    <!ENTITY owl "http://www.w3.org/2002/07/owl#" >
    <!ENTITY xsd "http://www.w3.org/2001/XMLSchema#" >
    <!ENTITY reve "http://data.eurecom.fr/ontology/reve#" >
    <!ENTITY rdfs "http://www.w3.org/2000/01/rdf-schema#" >
    <!ENTITY rdf "http://www.w3.org/1999/02/22-rdf-syntax-ns#" >
    <!ENTITY dcmi-terms "http://dublincore.org/documents/dcmi-terms/" >
]>


<rdf:RDF xmlns="http://data.eurecom.fr/ontology/reve#"
     xml:base="http://data.eurecom.fr/ontology/reve"
     xmlns:dcmi-terms="http://dublincore.org/documents/dcmi-terms/"
     xmlns:rdfs="http://www.w3.org/2000/01/rdf-schema#"
     xmlns:terms="http://purl.org/dc/terms/"
     xmlns:owl="http://www.w3.org/2002/07/owl#"
     xmlns:xsd="http://www.w3.org/2001/XMLSchema#"
     xmlns:rdf="http://www.w3.org/1999/02/22-rdf-syntax-ns#"
     xmlns:reve="http://data.eurecom.fr/ontology/reve#"
     xmlns:cc="http://web.resource.org/cc/"
     xmlns:vocab.sindice="http://vocab.sindice.net/">
    <owl:Ontology rdf:about="http://data.eurecom.fr/ontology/reve">
        <rdfs:label xml:lang="en">Research and Education Vocabulary for EURECOM</rdfs:label>
        <owl:versionInfo>1.0</owl:versionInfo>
        <rdfs:comment xml:lang="en">An ontology to describe students, courses, publications and researchers at Eurecom</rdfs:comment>
    </owl:Ontology>
    


    <!-- 
    ///////////////////////////////////////////////////////////////////////////////////////
    //
    // Annotation properties
    //
    ///////////////////////////////////////////////////////////////////////////////////////
     -->

    <owl:AnnotationProperty rdf:about="&owl;versionInfo"/>
    <owl:AnnotationProperty rdf:about="&rdfs;isDefinedBy"/>
    <owl:AnnotationProperty rdf:about="&rdfs;label"/>
    <owl:AnnotationProperty rdf:about="&rdfs;comment"/>
    


    <!-- 
    ///////////////////////////////////////////////////////////////////////////////////////
    //
    // Datatypes
    //
    ///////////////////////////////////////////////////////////////////////////////////////
     -->

    


    <!-- http://www.w3.org/2001/XMLSchema#date -->

    <rdfs:Datatype rdf:about="&xsd;date"/>
    


    <!-- http://www.w3.org/2001/XMLSchema#float -->

    <rdfs:Datatype rdf:about="&xsd;float"/>
    


    <!-- 
    ///////////////////////////////////////////////////////////////////////////////////////
    //
    // Object Properties
    //
    ///////////////////////////////////////////////////////////////////////////////////////
     -->

    


    <!-- http://data.eurecom.fr/ontology/reve#availableDuring -->

    <owl:ObjectProperty rdf:about="&reve;availableDuring">
        <rdfs:label xml:lang="en">available during</rdfs:label>
        <rdfs:label xml:lang="fr">disponible pendant</rdfs:label>
        <rdfs:comment xml:lang="en">Property referencing a semester during which the course is available</rdfs:comment>
        <rdfs:comment xml:lang="fr">Propriété faisant référence à un semestre pendant lequel le cours est disponible</rdfs:comment>
        <rdfs:isDefinedBy rdf:resource="http://data.eurecom.fr/ontology/"/>
        <rdfs:domain rdf:resource="&reve;Course"/>
        <rdfs:range rdf:resource="&reve;Semester"/>
        <owl:inverseOf rdf:resource="&reve;hasAvailableCourse"/>
    </owl:ObjectProperty>
    


    <!-- http://data.eurecom.fr/ontology/reve#hasAvailableCourse -->

    <owl:ObjectProperty rdf:about="&reve;hasAvailableCourse">
        <rdfs:label xml:lang="en">has available course</rdfs:label>
        <rdfs:label xml:lang="fr">a comme cours disponible</rdfs:label>
        <rdfs:comment xml:lang="en">Property referencing a course available during the semester</rdfs:comment>
        <rdfs:comment xml:lang="fr">Propriété faisant référence à un cours disponible pendant le semestre</rdfs:comment>
        <rdfs:isDefinedBy rdf:resource="http://data.eurecom.fr/ontology/"/>
        <rdfs:range rdf:resource="&reve;Course"/>
        <rdfs:domain rdf:resource="&reve;Semester"/>
    </owl:ObjectProperty>
    


    <!-- http://data.eurecom.fr/ontology/reve#hasConstituent -->

    <owl:ObjectProperty rdf:about="&reve;hasConstituent">
        <rdfs:label xml:lang="en">has constituent</rdfs:label>
        <rdfs:label xml:lang="fr">a pour constituant</rdfs:label>
        <rdfs:comment xml:lang="en">A course consists in several course sessions</rdfs:comment>
        <rdfs:comment xml:lang="fr">Un cours est constitué de plusieurs sessions de cours</rdfs:comment>
        <rdfs:isDefinedBy rdf:resource="http://data.eurecom.fr/ontology/"/>
        <rdfs:domain rdf:resource="&reve;Course"/>
        <rdfs:range rdf:resource="&reve;CourseSession"/>
    </owl:ObjectProperty>
    


    <!-- http://data.eurecom.fr/ontology/reve#hasCoordinator -->

    <owl:ObjectProperty rdf:about="&reve;hasCoordinator">
        <rdfs:label xml:lang="en">has coordinator</rdfs:label>
        <rdfs:label xml:lang="fr">a pour coordinateur</rdfs:label>
        <rdfs:comment xml:lang="en">Property referencing a person responsible for the track</rdfs:comment>
        <rdfs:comment xml:lang="fr">Propriété faisant référence à une personne responsable de la filière</rdfs:comment>
        <rdfs:isDefinedBy rdf:resource="http://data.eurecom.fr/ontology/"/>
        <rdfs:domain rdf:resource="&reve;Track"/>
        <owl:inverseOf rdf:resource="&reve;isCoordinatorOf"/>
        <rdfs:range rdf:resource="http://xmlns.com/foaf/0.1/Person"/>
    </owl:ObjectProperty>
    


    <!-- http://data.eurecom.fr/ontology/reve#hasCreditForTrack -->

    <owl:ObjectProperty rdf:about="&reve;hasCreditForTrack">
        <rdfs:label xml:lang="en">has credit for track</rdfs:label>
        <rdfs:label xml:lang="fr">Crédit pour la filière</rdfs:label>
        <rdfs:comment xml:lang="en">Property referencing to the credits for the successful completion of the course in a given track.</rdfs:comment>
        <rdfs:comment xml:lang="fr">Propriété faisant référence au nombre de crédits reçus pour la validation du cours dans une filière donnée.</rdfs:comment>
        <rdfs:domain rdf:resource="&reve;Course"/>
        <rdfs:range rdf:resource="&reve;CourseCreditForTrack"/>
    </owl:ObjectProperty>
    


    <!-- http://data.eurecom.fr/ontology/reve#hasDuration -->

    <owl:ObjectProperty rdf:about="&reve;hasDuration">
        <rdfs:label xml:lang="en">has duration</rdfs:label>
        <rdfs:comment xml:lang="en">Property referencing a semester in the curriculum.</rdfs:comment>
        <rdfs:domain rdf:resource="&reve;Curriculum"/>
        <rdfs:range rdf:resource="&reve;Semester"/>
        <owl:inverseOf rdf:resource="&reve;isDurationOf"/>
    </owl:ObjectProperty>
    


    <!-- http://data.eurecom.fr/ontology/reve#hasFreeCourse -->

    <owl:ObjectProperty rdf:about="&reve;hasFreeCourse">
        <rdfs:label xml:lang="en">has free course</rdfs:label>
        <rdfs:comment xml:lang="en">Property referencing a course considered free for the track</rdfs:comment>
        <rdfs:range rdf:resource="&reve;Course"/>
        <rdfs:domain rdf:resource="&reve;Track"/>
        <owl:inverseOf rdf:resource="&reve;isFreeFor"/>
    </owl:ObjectProperty>
    


    <!-- http://data.eurecom.fr/ontology/reve#hasMandatoryCourse -->

    <owl:ObjectProperty rdf:about="&reve;hasMandatoryCourse">
        <rdfs:label xml:lang="en">has mandatory course</rdfs:label>
        <rdfs:label xml:lang="fr">a comme cours obligatoire</rdfs:label>
        <rdfs:comment xml:lang="en">Property referencing a course considered mandatory for the track</rdfs:comment>
        <rdfs:comment xml:lang="fr">Propriété faisant référence à un cours considéré comme obligatoire pour la filière</rdfs:comment>
        <rdfs:isDefinedBy rdf:resource="http://data.eurecom.fr/ontology/"/>
        <rdfs:range rdf:resource="&reve;Course"/>
        <rdfs:domain rdf:resource="&reve;Track"/>
        <owl:inverseOf rdf:resource="&reve;isMandatoryFor"/>
    </owl:ObjectProperty>
    


    <!-- http://data.eurecom.fr/ontology/reve#hasOptionalCourse -->

    <owl:ObjectProperty rdf:about="&reve;hasOptionalCourse">
        <rdfs:label xml:lang="en">has optional course</rdfs:label>
        <rdfs:label xml:lang="fr">a comme cours optionnel</rdfs:label>
        <rdfs:comment xml:lang="en">Property referencing a course considered optional for the track</rdfs:comment>
        <rdfs:comment xml:lang="fr">Propriété faisant référence à un cours considéré comme optionnel pour la filière</rdfs:comment>
        <rdfs:isDefinedBy rdf:resource="http://data.eurecom.fr/ontology/"/>
        <rdfs:range rdf:resource="&reve;Course"/>
        <rdfs:domain rdf:resource="&reve;Track"/>
    </owl:ObjectProperty>
    


    <!-- http://data.eurecom.fr/ontology/reve#hasTrack -->

    <owl:ObjectProperty rdf:about="&reve;hasTrack">
        <rdfs:label xml:lang="en">has track</rdfs:label>
        <rdfs:label xml:lang="fr">filière</rdfs:label>
        <rdfs:comment xml:lang="en">Property referencing to a track in the (course, credit, track) relationship.</rdfs:comment>
        <rdfs:comment xml:lang="fr">Propriété faisant référence à la filière dans la relation (cours, crédit, filière).</rdfs:comment>
        <rdfs:domain rdf:resource="&reve;CourseCreditForTrack"/>
        <rdfs:range rdf:resource="&reve;Track"/>
        <owl:inverseOf rdf:resource="&reve;isTrackOf"/>
    </owl:ObjectProperty>
    


    <!-- http://data.eurecom.fr/ontology/reve#isConstituentOf -->

    <owl:ObjectProperty rdf:about="&reve;isConstituentOf">
        <rdfs:label xml:lang="en">is constituent of</rdfs:label>
        <rdfs:label xml:lang="fr">est un constituant de</rdfs:label>
        <rdfs:comment xml:lang="en">A course consists in several course sessions</rdfs:comment>
        <rdfs:comment xml:lang="fr">Un cours est constitué de plusieurs sessions de cours</rdfs:comment>
        <rdfs:isDefinedBy rdf:resource="http://data.eurecom.fr/ontology/"/>
        <rdfs:range rdf:resource="&reve;Course"/>
        <rdfs:domain rdf:resource="&reve;CourseSession"/>
        <owl:inverseOf rdf:resource="&reve;hasConstituent"/>
    </owl:ObjectProperty>
    


    <!-- http://data.eurecom.fr/ontology/reve#isCoordinatorOf -->

    <owl:ObjectProperty rdf:about="&reve;isCoordinatorOf">
        <rdfs:label xml:lang="en">is coordinator of</rdfs:label>
        <rdfs:label xml:lang="fr">est le coordinateur de</rdfs:label>
        <rdfs:comment xml:lang="en">Property referencing a track the person is responsible for</rdfs:comment>
        <rdfs:comment xml:lang="fr">Propriété faisant référence à une filière dont la personne est responsable</rdfs:comment>
        <rdfs:isDefinedBy rdf:resource="http://data.eurecom.fr/ontology/"/>
        <rdfs:range rdf:resource="&reve;Track"/>
        <rdfs:domain rdf:resource="http://xmlns.com/foaf/0.1/Person"/>
    </owl:ObjectProperty>
    


    <!-- http://data.eurecom.fr/ontology/reve#isCreditForCourse -->

    <owl:ObjectProperty rdf:about="&reve;isCreditForCourse">
        <rdfs:label xml:lang="en">is credit for course</rdfs:label>
        <rdfs:label xml:lang="fr">est le crédit pour le cours</rdfs:label>
        <rdfs:comment xml:lang="en">Property referencing the course in the (course, credit, track) relationship.</rdfs:comment>
        <rdfs:comment xml:lang="fr">Propriété faisant référence au cours dans la relation (cours, crédit, filière).</rdfs:comment>
        <rdfs:range rdf:resource="&reve;Course"/>
        <rdfs:domain rdf:resource="&reve;CourseCreditForTrack"/>
        <owl:inverseOf rdf:resource="&reve;hasCreditForTrack"/>
    </owl:ObjectProperty>
    


    <!-- http://data.eurecom.fr/ontology/reve#isDurationOf -->

    <owl:ObjectProperty rdf:about="&reve;isDurationOf">
        <rdfs:label xml:lang="en">is duration of</rdfs:label>
        <rdfs:comment xml:lang="en">Property referencing to a curriculum for which the semester is included</rdfs:comment>
        <rdfs:range rdf:resource="&reve;Curriculum"/>
        <rdfs:domain rdf:resource="&reve;Semester"/>
    </owl:ObjectProperty>
    


    <!-- http://data.eurecom.fr/ontology/reve#isFreeFor -->

    <owl:ObjectProperty rdf:about="&reve;isFreeFor">
        <rdfs:label xml:lang="en">is free for</rdfs:label>
        <rdfs:comment xml:lang="en">Property referencing a track for which the course is considered free.</rdfs:comment>
        <rdfs:domain rdf:resource="&reve;Course"/>
        <rdfs:range rdf:resource="&reve;Track"/>
    </owl:ObjectProperty>
    


    <!-- http://data.eurecom.fr/ontology/reve#isMandatoryFor -->

    <owl:ObjectProperty rdf:about="&reve;isMandatoryFor">
        <rdfs:label xml:lang="en">is mandatory for</rdfs:label>
        <rdfs:label xml:lang="fr">est obligatoire pour</rdfs:label>
        <rdfs:comment xml:lang="en">Property referencing a track for which the course is considered mandatory</rdfs:comment>
        <rdfs:comment xml:lang="fr">Propriété faisant référence à une filière pour laquelle le cours est considéré comme obligatoire</rdfs:comment>
        <rdfs:isDefinedBy rdf:resource="http://data.eurecom.fr/ontology/"/>
        <rdfs:domain rdf:resource="&reve;Course"/>
        <rdfs:range rdf:resource="&reve;Track"/>
    </owl:ObjectProperty>
    


    <!-- http://data.eurecom.fr/ontology/reve#isOptionalFor -->

    <owl:ObjectProperty rdf:about="&reve;isOptionalFor">
        <rdfs:label xml:lang="en">is optional for</rdfs:label>
        <rdfs:label xml:lang="fr">est optionnel pour</rdfs:label>
        <rdfs:comment xml:lang="en">Property referencing a track for which the course is considered optional</rdfs:comment>
        <rdfs:comment xml:lang="fr">Propriété faisant référence à une filière pour laquelle le cours est considéré comme optionnel</rdfs:comment>
        <rdfs:isDefinedBy rdf:resource="http://data.eurecom.fr/ontology/"/>
        <rdfs:domain rdf:resource="&reve;Course"/>
        <rdfs:range rdf:resource="&reve;Track"/>
        <owl:inverseOf rdf:resource="&reve;hasOptionalCourse"/>
    </owl:ObjectProperty>
    


    <!-- http://data.eurecom.fr/ontology/reve#isTrackOf -->

    <owl:ObjectProperty rdf:about="&reve;isTrackOf">
        <rdfs:label xml:lang="en">is track of</rdfs:label>
        <rdfs:label xml:lang="fr">est la filière de</rdfs:label>
        <rdfs:comment xml:lang="en">Property referencing to a (course, credit, track) relationship the track is involved in.</rdfs:comment>
        <rdfs:comment xml:lang="fr">Propriété faisant référence à une relation (cours, crédit, filière) dans laquelle la filière est impliquée.</rdfs:comment>
        <rdfs:range rdf:resource="&reve;CourseCreditForTrack"/>
        <rdfs:domain rdf:resource="&reve;Track"/>
    </owl:ObjectProperty>
    


    <!-- http://purl.org/dc/terms/type -->

    <owl:ObjectProperty rdf:about="&terms;type"/>
    


    <!-- http://web.resource.org/cc/license -->

    <owl:ObjectProperty rdf:about="&cc;license"/>
    


    <!-- http://web.resource.org/cc/permits -->

    <owl:ObjectProperty rdf:about="&cc;permits"/>
    


    <!-- http://web.resource.org/cc/requires -->

    <owl:ObjectProperty rdf:about="&cc;requires"/>
    


    <!-- 
    ///////////////////////////////////////////////////////////////////////////////////////
    //
    // Data properties
    //
    ///////////////////////////////////////////////////////////////////////////////////////
     -->

    


    <!-- http://data.eurecom.fr/ontology/reve#hasCredit -->

    <owl:DatatypeProperty rdf:about="&reve;hasCredit">
        <rdfs:label xml:lang="en">has credit</rdfs:label>
        <rdfs:label xml:lang="fr">crédit</rdfs:label>
        <rdfs:comment xml:lang="en">Data type property referencing the number of credits in the (course, credit, track) relationship.</rdfs:comment>
        <rdfs:comment xml:lang="fr">Attribut faisant référence au nombre de crédits dans la relation (cours, crédit, filière).</rdfs:comment>
        <rdfs:domain rdf:resource="&reve;CourseCreditForTrack"/>
        <rdfs:range rdf:resource="&xsd;float"/>
    </owl:DatatypeProperty>
    


    <!-- http://data.eurecom.fr/ontology/reve#referenceAtEurecom -->

    <owl:DatatypeProperty rdf:about="&reve;referenceAtEurecom">
        <rdfs:label xml:lang="en">reference at Eurecom</rdfs:label>
        <rdfs:label xml:lang="fr">référence Eurecom</rdfs:label>
        <rdfs:comment xml:lang="en">An article&apos;s reference in Eurecom&apos;s bibliographic repository.</rdfs:comment>
        <rdfs:comment xml:lang="fr">La référence d&apos;un article dans la base bibliographique d&apos;Eurecom.</rdfs:comment>
        <rdfs:isDefinedBy rdf:resource="http://data.eurecom.fr/ontology/"/>
        <rdfs:domain rdf:resource="http://xmlns.com/foaf/0.1/Document"/>
    </owl:DatatypeProperty>
    


    <!-- http://dublincore.org/documents/dcmi-terms/created -->

    <owl:DatatypeProperty rdf:about="&dcmi-terms;created"/>
    


    <!-- http://dublincore.org/documents/dcmi-terms/title -->

    <owl:DatatypeProperty rdf:about="&dcmi-terms;title"/>
    


    <!-- http://purl.org/dc/terms/issued -->

    <owl:DatatypeProperty rdf:about="&terms;issued"/>
    


    <!-- http://purl.org/dc/terms/rights -->

    <owl:DatatypeProperty rdf:about="&terms;rights"/>
    


    <!-- http://vocab.sindice.net/date -->

    <owl:DatatypeProperty rdf:about="&vocab.sindice;date"/>
    


    <!-- http://vocab.sindice.net/size -->

    <owl:DatatypeProperty rdf:about="&vocab.sindice;size"/>
    


    <!-- 
    ///////////////////////////////////////////////////////////////////////////////////////
    //
    // Classes
    //
    ///////////////////////////////////////////////////////////////////////////////////////
     -->

    


    <!-- http://data.eurecom.fr/ontology/reve#Alumnus -->

    <owl:Class rdf:about="&reve;Alumnus">
        <rdfs:label xml:lang="en">Alumnus</rdfs:label>
        <rdfs:label xml:lang="fr">Ancien élève</rdfs:label>
        <rdfs:subClassOf rdf:resource="http://purl.org/vocab/aiiso-roles/schema#Role"/>
        <rdfs:comment xml:lang="en">Holders of this role have graduated and received a PhD diploma or a Eurecom certificate</rdfs:comment>
        <rdfs:comment xml:lang="fr">Les titulaires de ce rôle ont fini un cursus à Eurecom et détiennent un diplôme de doctorat ou une certification Eurecom</rdfs:comment>
        <rdfs:isDefinedBy rdf:resource="http://data.eurecom.fr/ontology/"/>
    </owl:Class>
    


    <!-- http://data.eurecom.fr/ontology/reve#Attendee -->

    <owl:Class rdf:about="&reve;Attendee">
        <rdfs:label xml:lang="en">Attendee</rdfs:label>
        <rdfs:label xml:lang="fr">Participant</rdfs:label>
        <rdfs:subClassOf rdf:resource="http://purl.org/vocab/aiiso-roles/schema#Role"/>
        <rdfs:comment xml:lang="en">Holders of this role have registered for one or several courses</rdfs:comment>
        <rdfs:comment xml:lang="fr">Les titulaires de ce rôle sont inscrits à un ou plusieurs cours</rdfs:comment>
        <rdfs:isDefinedBy rdf:resource="http://data.eurecom.fr/ontology/"/>
    </owl:Class>
    


    <!-- http://data.eurecom.fr/ontology/reve#Course -->

    <owl:Class rdf:about="&reve;Course">
        <rdfs:label xml:lang="en">Course</rdfs:label>
        <rdfs:label xml:lang="fr">Cours</rdfs:label>
        <owl:equivalentClass rdf:resource="http://purl.org/vocab/aiiso/schema#Course"/>
        <rdfs:comment xml:lang="en">A teaching unit. A course is composed of several course sessions.</rdfs:comment>
        <rdfs:comment xml:lang="fr">Une unité d&apos;enseignement. Un cours est composé de plusieurs sessions de cours.</rdfs:comment>
        <rdfs:isDefinedBy rdf:resource="http://data.eurecom.fr/ontology/"/>
    </owl:Class>
    


    <!-- http://data.eurecom.fr/ontology/reve#CourseCreditForTrack -->

    <owl:Class rdf:about="&reve;CourseCreditForTrack">
        <rdfs:label xml:lang="en">Course credit for track.</rdfs:label>
        <rdfs:label xml:lang="fr">Crédit du cours pour la filière.</rdfs:label>
        <rdfs:comment xml:lang="en">A container for n-ary relationship for Course, Track and credits number.</rdfs:comment>
        <rdfs:comment xml:lang="fr">Un contenant de la relation n-aire pour le cours, la filière et le nombre de crédits.</rdfs:comment>
    </owl:Class>
    


    <!-- http://data.eurecom.fr/ontology/reve#CourseSession -->

    <owl:Class rdf:about="&reve;CourseSession">
        <rdfs:label xml:lang="en">Course session</rdfs:label>
        <rdfs:label xml:lang="fr">Session de cours</rdfs:label>
        <rdfs:subClassOf rdf:resource="http://linkedevents.org/ontology/Event"/>
        <rdfs:comment xml:lang="en">A course session is a ponctual event on which teacher and students gather, for a given course.</rdfs:comment>
        <rdfs:comment xml:lang="fr">Une session de cours est un évènement ponctuel qui rassemble professeur et élèves en un lieu donné, au sujet d&apos;un cours.</rdfs:comment>
        <rdfs:isDefinedBy rdf:resource="http://data.eurecom.fr/ontology/"/>
    </owl:Class>
    


    <!-- http://data.eurecom.fr/ontology/reve#Curriculum -->

    <owl:Class rdf:about="&reve;Curriculum">
        <rdfs:label xml:lang="en">Curriculum</rdfs:label>
        <rdfs:label xml:lang="fr">Formation</rdfs:label>
        <rdfs:comment xml:lang="en">A curriculum is a title of a training period offered at Eurecom which consists of credits compatible with the LMD European standard.
Eurecom supports four types of curriculum, which is Engineering, Master of science, Post Master degree and doctoral program.</rdfs:comment>
        <rdfs:comment xml:lang="fr">Une formation est une période d&apos;étude proposée par Eurecom comprenant des crédits compatibles au système LMD
Eurecom propose quatre types of formation, qui sont ingénieurie, master international, ingénieur de spécialisation et le programme doctoral. </rdfs:comment>
    </owl:Class>
    


    <!-- http://data.eurecom.fr/ontology/reve#DoctoralStudent -->

    <owl:Class rdf:about="&reve;DoctoralStudent">
        <rdfs:label xml:lang="en">Doctoral student</rdfs:label>
        <rdfs:label xml:lang="fr">Doctorant</rdfs:label>
        <rdfs:subClassOf rdf:resource="http://purl.org/vocab/aiiso-roles/schema#Role"/>
        <rdfs:comment xml:lang="en">Holders of this role are students doing a PhD thesis.</rdfs:comment>
        <rdfs:comment xml:lang="fr">Les titulaires de ce rôle sont les étudiants effectuant une thèse de doctorat.</rdfs:comment>
        <rdfs:isDefinedBy rdf:resource="http://data.eurecom.fr/ontology/"/>
    </owl:Class>
    


    <!-- http://data.eurecom.fr/ontology/reve#GeneralCourse -->

    <owl:Class rdf:about="&reve;GeneralCourse">
        <rdfs:label xml:lang="en">General course</rdfs:label>
        <rdfs:label xml:lang="fr">Cours d&apos;enseignement général</rdfs:label>
        <rdfs:subClassOf rdf:resource="&reve;Course"/>
        <rdfs:comment xml:lang="en">A course which brings knowledge in law, economy, or management</rdfs:comment>
        <rdfs:comment xml:lang="fr">Un cours qui apporte des connaissances en droit, en économie, ou en gestion</rdfs:comment>
        <rdfs:isDefinedBy rdf:resource="http://data.eurecom.fr/ontology/"/>
    </owl:Class>
    


    <!-- http://data.eurecom.fr/ontology/reve#LanguageCourse -->

    <owl:Class rdf:about="&reve;LanguageCourse">
        <rdfs:label xml:lang="en">Language course</rdfs:label>
        <rdfs:label xml:lang="fr">Cours de langue</rdfs:label>
        <rdfs:subClassOf rdf:resource="&reve;Course"/>
        <owl:disjointWith rdf:resource="&reve;TechnicalCourse"/>
        <rdfs:comment xml:lang="en">A course in which one learns a language other than one&apos;s native language</rdfs:comment>
        <rdfs:comment xml:lang="fr">Un cours où l&apos;on apprend à s&apos;exprimer dans une autre langue que la sienne</rdfs:comment>
        <rdfs:isDefinedBy rdf:resource="http://data.eurecom.fr/ontology/"/>
    </owl:Class>
    


    <!-- http://data.eurecom.fr/ontology/reve#ResearchUnit -->

    <owl:Class rdf:about="&reve;ResearchUnit">
        <rdfs:label xml:lang="en">Research unit</rdfs:label>
        <rdfs:label xml:lang="fr">Unité de recherche</rdfs:label>
        <owl:equivalentClass rdf:resource="http://purl.org/vocab/aiiso/schema#ResearchGroup"/>
        <rdfs:subClassOf rdf:resource="http://xmlns.com/foaf/0.1/Group"/>
        <rdfs:comment xml:lang="en">A Research Unit is a group dedicated to research at Eurecom, and there are three of them.</rdfs:comment>
        <rdfs:comment xml:lang="fr">Une unité de recherche est un groupe dédié à la recherche à Eurecom. Il y en a trois.</rdfs:comment>
        <rdfs:isDefinedBy rdf:resource="http://data.eurecom.fr/ontology/"/>
    </owl:Class>
    


    <!-- http://data.eurecom.fr/ontology/reve#Researcher -->

    <owl:Class rdf:about="&reve;Researcher">
        <rdfs:label xml:lang="en">Researcher</rdfs:label>
        <rdfs:label xml:lang="fr">Chercheur</rdfs:label>
        <rdfs:subClassOf rdf:resource="http://purl.org/vocab/aiiso-roles/schema#Role"/>
        <owl:disjointWith rdf:resource="&reve;Student"/>
        <rdfs:comment xml:lang="en">Holders of this role do research.</rdfs:comment>
        <rdfs:comment xml:lang="fr">Les titulaires de ce rôle effectuent des recherches.</rdfs:comment>
        <rdfs:isDefinedBy rdf:resource="http://data.eurecom.fr/ontology/"/>
    </owl:Class>
    


    <!-- http://data.eurecom.fr/ontology/reve#Semester -->

    <owl:Class rdf:about="&reve;Semester">
        <rdfs:label xml:lang="en">Semester</rdfs:label>
        <rdfs:label xml:lang="fr">Semestre</rdfs:label>
        <rdfs:comment xml:lang="en">A semester, from the administrative point of view : it typically ranges from the beginning of October to the middle of February, or from the beginning of March to the end of June. It has a catalog of courses attached to it.</rdfs:comment>
        <rdfs:comment xml:lang="fr">Un semestre, du point de vue administratif : typiquement, il s&apos;étend du début du mois d&apos;octobre à la mi-février, ou bien de mars à la fin juin. Un catalogue de cours y est rattaché.</rdfs:comment>
        <rdfs:isDefinedBy rdf:resource="http://data.eurecom.fr/ontology/"/>
    </owl:Class>
    


    <!-- http://data.eurecom.fr/ontology/reve#Staff -->

    <owl:Class rdf:about="&reve;Staff">
        <rdfs:label xml:lang="en">Staff</rdfs:label>
        <rdfs:label xml:lang="fr">Employé</rdfs:label>
        <rdfs:subClassOf rdf:resource="http://purl.org/vocab/aiiso-roles/schema#Role"/>
        <rdfs:comment xml:lang="en">Holders of this role receive a salary from Eurecom.</rdfs:comment>
        <rdfs:comment xml:lang="fr">Les titulaires de ce rôle reçoivent un salaire d&apos;Eurecom.</rdfs:comment>
        <rdfs:isDefinedBy rdf:resource="http://data.eurecom.fr/ontology/"/>
    </owl:Class>
    


    <!-- http://data.eurecom.fr/ontology/reve#Student -->

    <owl:Class rdf:about="&reve;Student">
        <rdfs:label xml:lang="en">Student</rdfs:label>
        <rdfs:label xml:lang="fr">Etudiant</rdfs:label>
        <rdfs:subClassOf rdf:resource="http://purl.org/vocab/aiiso-roles/schema#Role"/>
        <owl:disjointWith rdf:resource="&reve;Teacher"/>
        <rdfs:comment xml:lang="en">Holders of this role are enrolled at a university.</rdfs:comment>
        <rdfs:comment xml:lang="fr">Les titulaires de ce rôle sont engagés dans un cursus d&apos;enseignement supérieur.</rdfs:comment>
        <rdfs:isDefinedBy rdf:resource="http://data.eurecom.fr/ontology/"/>
    </owl:Class>
    


    <!-- http://data.eurecom.fr/ontology/reve#Teacher -->

    <owl:Class rdf:about="&reve;Teacher">
        <rdfs:label xml:lang="en">Teacher</rdfs:label>
        <rdfs:label xml:lang="fr">Enseignant</rdfs:label>
        <rdfs:subClassOf rdf:resource="http://purl.org/vocab/aiiso-roles/schema#Role"/>
        <rdfs:comment xml:lang="en">Holders of this role teach one or several courses.</rdfs:comment>
        <rdfs:comment xml:lang="fr">Les titulaires de ce rôle enseignent un ou plusieurs cours.</rdfs:comment>
        <rdfs:isDefinedBy rdf:resource="http://data.eurecom.fr/ontology/"/>
    </owl:Class>
    


    <!-- http://data.eurecom.fr/ontology/reve#TechnicalCourse -->

    <owl:Class rdf:about="&reve;TechnicalCourse">
        <rdfs:label xml:lang="en">Technical course</rdfs:label>
        <rdfs:label xml:lang="fr">Cours d&apos;enseignement technique</rdfs:label>
        <rdfs:subClassOf rdf:resource="&reve;Course"/>
        <rdfs:comment xml:lang="en">A course which brings scientific knowledge in one of the domains of expertise of Eurecom</rdfs:comment>
        <rdfs:comment xml:lang="fr">Un cours qui apporte des connaissances scientifiques dans l&apos;un des domaines d&apos;expertise d&apos;Eurecom.</rdfs:comment>
        <rdfs:isDefinedBy rdf:resource="http://data.eurecom.fr/ontology/"/>
    </owl:Class>
    


    <!-- http://data.eurecom.fr/ontology/reve#Track -->

    <owl:Class rdf:about="&reve;Track">
        <rdfs:label xml:lang="en">Track</rdfs:label>
        <rdfs:label xml:lang="fr">Filière</rdfs:label>
        <rdfs:subClassOf rdf:resource="http://purl.org/vocab/aiiso/schema#KnowledgeGrouping"/>
        <rdfs:comment xml:lang="en">A set of mandatory and optional courses, built around a common domain. To help students select their courses, the curriculum is organized around 7 teaching tracks. Each track includes core courses, restrictive elective courses, and free elective courses that students are entirely free to choose from (except for languages).</rdfs:comment>
        <rdfs:comment xml:lang="fr">Un ensemble de cours obligatoires et optionnels, contruit autour d&apos;un même domaine. Pour aider les étudiants à choisir leur cours, le cursus est organisé autour de 7 filières d&apos;enseignement. Chaque filière comprend des cours obligatoires, des cours à choisir dans un menu et des cours à choix entièrement libres (à l&apos;exception des cours de langues vivantes).</rdfs:comment>
        <rdfs:isDefinedBy rdf:resource="http://data.eurecom.fr/ontology/"/>
    </owl:Class>
    


    <!-- http://data.eurecom.fr/ontology/reve#VisitingScientist -->

    <owl:Class rdf:about="&reve;VisitingScientist">
        <rdfs:label xml:lang="en">Visiting scientist</rdfs:label>
        <rdfs:label xml:lang="fr">Visiteur scientifique</rdfs:label>
        <rdfs:subClassOf rdf:resource="http://purl.org/vocab/aiiso-roles/schema#Role"/>
        <rdfs:comment xml:lang="en">Holders of this role are researchers welcomed at Eurecom for a certain duration</rdfs:comment>
        <rdfs:comment xml:lang="fr">Les titulaires de ce rôle sont des chercheurs reçus à Eurecom pour une durée déterminée</rdfs:comment>
        <rdfs:isDefinedBy rdf:resource="http://data.eurecom.fr/ontology/"/>
    </owl:Class>
    


    <!-- http://linkedevents.org/ontology/Event -->

    <owl:Class rdf:about="http://linkedevents.org/ontology/Event"/>
    


    <!-- http://purl.org/vocab/aiiso-roles/schema#Role -->

    <owl:Class rdf:about="http://purl.org/vocab/aiiso-roles/schema#Role"/>
    


    <!-- http://purl.org/vocab/aiiso/schema#Course -->

    <owl:Class rdf:about="http://purl.org/vocab/aiiso/schema#Course"/>
    


    <!-- http://purl.org/vocab/aiiso/schema#KnowledgeGrouping -->

    <owl:Class rdf:about="http://purl.org/vocab/aiiso/schema#KnowledgeGrouping"/>
    


    <!-- http://purl.org/vocab/aiiso/schema#ResearchGroup -->

    <owl:Class rdf:about="http://purl.org/vocab/aiiso/schema#ResearchGroup"/>
    


    <!-- http://web.resource.org/cc/License -->

    <owl:Class rdf:about="&cc;License"/>
    


    <!-- http://web.resource.org/cc/Work -->

    <owl:Class rdf:about="&cc;Work"/>
    


    <!-- http://xmlns.com/foaf/0.1/Document -->

    <owl:Class rdf:about="http://xmlns.com/foaf/0.1/Document"/>
    


    <!-- http://xmlns.com/foaf/0.1/Group -->

    <owl:Class rdf:about="http://xmlns.com/foaf/0.1/Group"/>
    


    <!-- http://xmlns.com/foaf/0.1/Person -->

    <owl:Class rdf:about="http://xmlns.com/foaf/0.1/Person"/>
    


    <!-- 
    ///////////////////////////////////////////////////////////////////////////////////////
    //
    // Individuals
    //
    ///////////////////////////////////////////////////////////////////////////////////////
     -->

    


    <!-- file:/C:/Users/Ghislain/Documents/Ghislain/data-eurecom-fr/REVE%20ontology/reve_1.0.rdf -->

    <owl:NamedIndividual rdf:about="file:/C:/Users/Ghislain/Documents/Ghislain/data-eurecom-fr/REVE%20ontology/reve_1.0.rdf">
        <rdf:type rdf:resource="&cc;Work"/>
        <cc:license rdf:resource="http://creativecommons.org/licenses/by/1.0/"/>
        <terms:type rdf:resource="http://purl.org/dc/dcmitype/Text"/>
    </owl:NamedIndividual>
    


    <!-- http://any23.org/tmp/ -->

    <owl:Thing rdf:about="http://any23.org/tmp/">
        <rdf:type rdf:resource="&owl;NamedIndividual"/>
        <vocab.sindice:size rdf:datatype="&xsd;int">296</vocab.sindice:size>
        <vocab.sindice:date>2012-01-19T15:48:03+00:00</vocab.sindice:date>
    </owl:Thing>
    


    <!-- http://creativecommons.org/licenses/by/1.0/ -->

    <owl:NamedIndividual rdf:about="http://creativecommons.org/licenses/by/1.0/">
        <rdf:type rdf:resource="&cc;License"/>
        <cc:requires rdf:resource="&cc;Attribution"/>
        <cc:permits rdf:resource="&cc;DerivativeWorks"/>
        <cc:permits rdf:resource="&cc;Distribution"/>
        <cc:requires rdf:resource="&cc;Notice"/>
        <cc:permits rdf:resource="&cc;Reproduction"/>
    </owl:NamedIndividual>
    


    <!-- http://data.eurecom.fr/ontology/reve -->

    <owl:Thing rdf:about="http://data.eurecom.fr/ontology/reve">
        <rdf:type rdf:resource="&owl;NamedIndividual"/>
        <dcmi-terms:created rdf:datatype="&xsd;date">2011-12-09</dcmi-terms:created>
        <terms:issued rdf:datatype="&xsd;date">2012-01-19</terms:issued>
        <terms:rights>Copyright 2012 EURECOM</terms:rights>
        <dcmi-terms:title xml:lang="en">Research and Education Vocabulary for Eurecom</dcmi-terms:title>
    </owl:Thing>
    


    <!-- http://data.eurecom.fr/ontology/reve#doctoralProgram -->

    <owl:NamedIndividual rdf:about="&reve;doctoralProgram">
        <rdf:type rdf:resource="&reve;Curriculum"/>
        <rdfs:label>doctoral program</rdfs:label>
    </owl:NamedIndividual>
    


    <!-- http://data.eurecom.fr/ontology/reve#engineering -->

    <owl:NamedIndividual rdf:about="&reve;engineering">
        <rdf:type rdf:resource="&reve;Curriculum"/>
        <rdfs:label>engineering</rdfs:label>
    </owl:NamedIndividual>
    


    <!-- http://data.eurecom.fr/ontology/reve#fall1 -->

    <owl:NamedIndividual rdf:about="&reve;fall1">
        <rdf:type rdf:resource="&reve;Semester"/>
        <rdfs:label>fall1</rdfs:label>
        <rdfs:comment>The first semester of engineering program.</rdfs:comment>
    </owl:NamedIndividual>
    


    <!-- http://data.eurecom.fr/ontology/reve#fall2 -->

    <owl:NamedIndividual rdf:about="&reve;fall2">
        <rdf:type rdf:resource="&reve;Semester"/>
        <rdfs:label>fall2</rdfs:label>
        <rdfs:comment>The third semester of engineering program.</rdfs:comment>
    </owl:NamedIndividual>
    


    <!-- http://data.eurecom.fr/ontology/reve#internship -->

    <owl:NamedIndividual rdf:about="&reve;internship">
        <rdf:type rdf:resource="&reve;Semester"/>
        <rdfs:label>inter</rdfs:label>
        <rdfs:comment>The internship semester of engineering program.</rdfs:comment>
    </owl:NamedIndividual>
    


    <!-- http://data.eurecom.fr/ontology/reve#masterOfScience -->

    <owl:NamedIndividual rdf:about="&reve;masterOfScience">
        <rdf:type rdf:resource="&reve;Curriculum"/>
        <rdfs:label>master of science</rdfs:label>
    </owl:NamedIndividual>
    


    <!-- http://data.eurecom.fr/ontology/reve#postMaster -->

    <owl:NamedIndividual rdf:about="&reve;postMaster">
        <rdf:type rdf:resource="&reve;Curriculum"/>
        <rdfs:label>post master</rdfs:label>
    </owl:NamedIndividual>
    


    <!-- http://data.eurecom.fr/ontology/reve#spring -->

    <owl:NamedIndividual rdf:about="&reve;spring">
        <rdf:type rdf:resource="&reve;Semester"/>
        <rdfs:label>spring</rdfs:label>
        <rdfs:comment>The second semester of engineering program.</rdfs:comment>
    </owl:NamedIndividual>
    


    <!-- http://purl.org/dc/dcmitype/Text -->

    <owl:Thing rdf:about="http://purl.org/dc/dcmitype/Text">
        <rdf:type rdf:resource="&owl;NamedIndividual"/>
    </owl:Thing>
    


    <!-- http://web.resource.org/cc/Attribution -->

    <owl:Thing rdf:about="&cc;Attribution">
        <rdf:type rdf:resource="&owl;NamedIndividual"/>
    </owl:Thing>
    


    <!-- http://web.resource.org/cc/DerivativeWorks -->

    <owl:Thing rdf:about="&cc;DerivativeWorks">
        <rdf:type rdf:resource="&owl;NamedIndividual"/>
    </owl:Thing>
    


    <!-- http://web.resource.org/cc/Distribution -->

    <owl:Thing rdf:about="&cc;Distribution">
        <rdf:type rdf:resource="&owl;NamedIndividual"/>
    </owl:Thing>
    


    <!-- http://web.resource.org/cc/Notice -->

    <owl:Thing rdf:about="&cc;Notice">
        <rdf:type rdf:resource="&owl;NamedIndividual"/>
    </owl:Thing>
    


    <!-- http://web.resource.org/cc/Reproduction -->

    <owl:Thing rdf:about="&cc;Reproduction">
        <rdf:type rdf:resource="&owl;NamedIndividual"/>
    </owl:Thing>
</rdf:RDF>



<!-- Generated by the OWL API (version 3.3.1957) http://owlapi.sourceforge.net -->

